coq/CoqArithUtils.v
@@ -1,0 +1,458 @@
+(** The Coq module [ArithUtils] contains arithmetic related lemmas
+    that help in proving the properties of interest in the formalization.
+
+    - @author Anonymized
+    - @author Anonymized
+    - @author Anonymized
+    - @author Anonymized
+
+*)
+
+Require Import ZArith.
+Require Import Lia.
+Require Import Int63.Sint63.
+Require Import Ascii String Coq.Strings.Byte.
+Require Import Lists.List.
+Import ListNotations.
+
+
+Lemma to_Z_of_nat:
+  forall (n:nat),
+    (Z.of_nat n < wB / 2)%Z ->
+    to_Z (Int63.Uint63.of_nat n) = Z.of_nat n.
+Proof.
+  intros.
+  rewrite of_Z_spec.
+  rewrite cmod_small;  lia.
+Qed.
+
+
+
+  
+Lemma of_nat_succ:
+  forall n,
+    (Z.of_nat (S n) < wB / 2)%Z ->
+    Int63.Uint63.of_nat (S n) = (1 + Int63.Uint63.of_nat n)%sint63.
+Proof.
+  induction n.
+  * intros. simpl.
+    now cbv.
+  * intros.
+    apply to_Z_inj.
+    rewrite IHn; try lia.
+    rewrite add_spec.
+    rewrite add_spec.
+    rewrite to_Z_of_nat by lia.
+    replace (S (S n)) with (1 + (1 + n)) by lia.
+    rewrite Nat2Z.inj_add.
+    rewrite Nat2Z.inj_add.
+    rewrite Nat2Z.inj_succ in H.
+    rewrite Nat2Z.inj_succ in H.
+    replace (Z.of_nat 1) with 1%Z by now cbv.
+    replace (to_Z 1) with 1%Z by now cbv.
+    rewrite cmod_small.
+    ** rewrite to_Z_of_nat by lia.
+       rewrite cmod_small; try lia.
+    ** rewrite to_Z_of_nat by lia.
+      rewrite cmod_small; try lia.
+Qed.
+
+Lemma of_nat_plus:
+  forall n m,
+    (Z.of_nat (n + m) < wB / 2)%Z ->
+    Int63.Uint63.of_nat (n + m)%nat = ((Int63.Uint63.of_nat n) + (Int63.Uint63.of_nat m))%uint63.
+Proof.
+  induction n.
+  * intros.
+    simpl.
+    rewrite add_of_Z.
+    simpl.
+    rewrite of_Z_spec.
+    now rewrite of_Z_cmod.
+  * intros.
+    rewrite plus_Sn_m.
+    rewrite of_nat_succ by lia.
+    rewrite of_nat_succ by lia.
+    rewrite IHn by lia.
+    now rewrite add_assoc.
+Qed.
+
+
+Lemma of_nat_minus:
+  forall n m,
+    (Z.of_nat n < wB / 2)%Z ->
+    m <= n ->
+    Int63.Uint63.of_nat (n - m)%nat = ((Int63.Uint63.of_nat n) - (Int63.Uint63.of_nat m))%uint63.
+Proof.
+  induction n.
+  * intros.
+    apply Nat.le_0_r in H0.
+    subst m.
+    now simpl.
+  * intros.
+    assert (1 + Z.of_nat  n < wB / 2)%Z. {
+      replace (S n) with (n + 1) in H by lia. 
+      rewrite Nat2Z.inj_add in H.
+      simpl in H.
+      lia.
+    }
+    destruct (le_gt_dec (S n) m).
+    ** assert (m = S n) by lia.
+       subst m.
+       rewrite Nat.sub_diag.
+       rewrite sub_of_Z.
+       rewrite Z.sub_diag.
+       now simpl. 
+    ** assert (m <= n) by lia.
+      rewrite Nat.sub_succ_l by lia.
+       rewrite of_nat_succ by lia.
+       rewrite of_nat_succ by lia.
+       rewrite IHn by lia.
+       assert (Z.of_nat m <= Z.of_nat n)%Z by auto using inj_le.
+       assert (to_Z (Int63.Uint63.of_nat m) >= 0)%Z. {
+         rewrite of_Z_spec.
+         rewrite cmod_small; lia.
+       }
+       apply  to_Z_inj.
+       rewrite add_spec.
+       rewrite sub_spec.
+       rewrite sub_spec.
+       rewrite add_spec.
+       replace (to_Z 1) with 1%Z by now cbv.
+       rewrite to_Z_of_nat by lia.
+       rewrite to_Z_of_nat by lia.
+       rewrite cmod_small.
+       *** rewrite cmod_small; try lia.
+           rewrite cmod_small; try lia.
+           rewrite cmod_small; try lia.
+           rewrite cmod_small; try lia.
+       *** rewrite cmod_small; try lia.
+Qed.
+
+
+Lemma zero_leq_max_int:
+  (0 <= to_Z max_int)%Z.
+Proof.
+  replace 0%Z with (to_Z 0) by now simpl.
+  apply to_Z_bounded.
+Qed.
+
+
+Lemma abs_int_low:
+  (to_Z min_int < 0)%Z.
+Proof.
+  now compute.
+Qed.
+
+Definition is_one_byte (n:int) := (0 <= (to_Z n) <= 2^8 - 1)%Z.
+
+(** A predicate to check if the integer [n] fits in two octets. *)
+Definition is_two_byte (n:int) := (0 <= (to_Z n) <= 2^16 - 1)%Z.
+
+Definition is_one_byte_sint (n: int): bool :=
+  (0 <=? n)%sint63 && (n <? 256)%sint63.
+
+Definition is_two_byte_sint (n: int): bool :=
+  (0 <=? n)%sint63 && (n <? 65536)%sint63.
+
+Lemma is_one_byte_non_negative:
+  forall n, is_one_byte n -> (0 <=? to_Z n)%Z = true.
+Proof.
+  intros.
+  unfold is_one_byte in H.
+  apply Z.leb_le.
+  now apply H.
+Qed.
+
+Lemma is_one_byte_negative:
+  forall n, is_one_byte n -> (to_Z n <? 0)%Z = false.
+Proof.
+  intros.
+  unfold is_one_byte in H.
+  now apply Z.ltb_ge.
+Qed.
+
+Lemma is_two_byte_non_negative:
+  forall n, is_two_byte n -> (0 <=? to_Z n)%Z = true.
+Proof.
+  intros.
+  unfold is_two_byte in H.
+  apply Z.leb_le.
+  now apply H.
+Qed.
+
+Lemma is_two_byte_negative:
+  forall n, is_two_byte n -> (to_Z n <? 0)%Z = false.
+Proof.
+  intros.
+  unfold is_two_byte in H.
+  now apply Z.ltb_ge.
+Qed.
+
+(** Create a one byte out of an integer [no] in the range 0..255.
+
+ It should not be used for integers outside the range. *)
+
+(** Create a two bytes out of an integer [no] in the range 0..65535.
+
+ It should not be used for integers outside the range. *)
+Definition two_byte_of_int (no:int) :=
+  let hibyte := (to_Z (no / 256%uint63))%Z in
+  let lobyte := (to_Z (no mod 256%uint63))%Z in
+  if (256 <=? hibyte)%Z
+  then (string_of_list_ascii ["000"%char; "000"%char])
+  else (string_of_list_ascii [(ascii_of_nat (Z.to_nat hibyte));
+                              (ascii_of_nat (Z.to_nat lobyte))]).
+
+
+Lemma is_two_byte_leq256:
+  forall no,
+    is_two_byte no ->      
+    (256 <=? to_Z (no / 256%sint63))%Z= false.
+Proof.
+  intros.
+  unfold is_two_byte in H.
+  apply Z.leb_nle.
+  intro.
+  destruct H.
+  apply Z.le_ge in H0.
+  assert (256 > 0)%Z by lia.
+  rewrite div_spec in H0.
+  * rewrite Z.quot_div_nonneg in H0;[|auto|now compute]; try lia.
+    apply Z.le_ge in H1.
+    eapply Z_div_ge in H1; eauto.
+    replace (to_Z 256) with (256%Z) in H0 by now compute.
+    simpl in H1.
+    replace (65535 / 256)%Z with 255%Z in H1 by now compute.
+    lia.
+  * right;now compute.
+Qed.
+
+Lemma split_two_bytes_eq_init:
+  forall (no:int),
+    is_two_byte no ->
+    (of_Z           
+       (Z.of_nat   
+          (256 * nat_of_ascii (ascii_of_nat (Z.to_nat (to_Z (no / 256)))) +
+             nat_of_ascii (ascii_of_nat (Z.to_nat (to_Z (no mod 256))))))) = no.
+Proof.
+  intros.
+  unfold is_two_byte in H.
+  assert (to_Z 256 = 256%Z) as to256. { 
+    now compute.
+  }
+  rewrite nat_ascii_embedding.
+  rewrite nat_ascii_embedding.  
+  * rewrite Nat2Z.inj_add.
+    replace 256  with (Z.to_nat 256%Z); [|now compute].
+    rewrite div_spec;[|right;now compute].
+    rewrite Z.quot_div_nonneg; try lia. 
+    rewrite <- Z2Nat.inj_mul;try apply Z.div_pos; try lia. 
+    rewrite Z2Nat.id.
+    rewrite Z2Nat.id.
+    ** rewrite mod_spec.
+       rewrite Z.rem_mod_nonneg; try lia.    
+       rewrite to256.   
+       rewrite <- Z_div_mod_eq_full.
+       now rewrite of_to_Z.
+    ** rewrite mod_spec.
+       rewrite Z.rem_mod_nonneg; try lia.
+       rewrite to256.
+       apply Z_mod_nonneg_nonneg;lia.
+    ** apply Ztac.mul_le;try lia.
+       apply Z.div_pos; try lia.
+  * rewrite mod_spec.
+    rewrite Z.rem_mod_nonneg; try lia.
+    rewrite to256.
+    rewrite Z2Nat.inj_mod;try lia.
+    replace (Z.to_nat 256) with 256;[|now compute].
+    apply Nat.mod_bound_pos; try lia.
+  * replace 256 with (Z.to_nat 256%Z) by lia. 
+    apply Z2Nat.inj_lt; try lia. 
+    ** rewrite div_spec;[|right;now compute].
+       rewrite Z.quot_div_nonneg; try lia. 
+       rewrite to256.
+       apply Z_div_nonneg_nonneg; try lia.
+    ** rewrite div_spec;[|right;now compute].
+       rewrite Z.quot_div_nonneg; [|lia|lia].
+       rewrite to256.
+       apply Z.div_lt_upper_bound; try lia.
+Qed.
+
+
+
+
+Lemma max_zero_rem:
+  forall no,
+    (0 <= to_Z no <= 2 ^ 16 - 1)%Z ->
+    Z.max 0 (Z.rem (to_Z no) (to_Z 256)) =  (Z.rem (to_Z no) (to_Z 256)).
+Proof.
+  intros.
+  decompose [and] H;clear H.
+  rewrite Z.max_r;auto.
+  apply Z.rem_bound_pos;eauto.
+  now compute.
+Qed.
+
+Lemma max_zero_quot:
+  forall no,
+    (0 <= to_Z no <= 2 ^ 16 - 1)%Z ->
+    (Z.max 0 (to_Z no  ÷ to_Z 256) = (to_Z no  ÷ to_Z 256))%Z.
+Proof.
+  intros.
+  decompose [and] H;clear H.
+  rewrite Z.max_r;auto.
+  apply Z.quot_le_lower_bound; auto.
+  now compute.
+Qed.
+
+Lemma rem_of_Z:
+  forall x y,
+    of_Z (Z.rem (to_Z x) (to_Z y)) = (x mod y)%sint63.
+Proof.
+  intros.
+  rewrite <- mod_spec.
+  now rewrite of_to_Z.
+Qed.
+  
+Lemma quot_of_Z:
+  forall x y,
+     x <> min_int \/ to_Z y <> (-1)%Z ->
+    of_Z (to_Z x  ÷ to_Z y) = (x / y)%sint63.
+Proof.
+  intros.
+  rewrite <- div_spec.
+  * now rewrite of_to_Z.
+  * destruct H.
+    ** left.
+       intro.
+       apply H.
+       now apply to_Z_inj.
+    ** now right.
+Qed.
+
+
+Lemma split_two_bytes_eq_init_int:
+  forall (no:int),
+    is_two_byte no ->
+    (256 * Int63.Uint63.of_nat (nat_of_ascii (ascii_of_nat (Z.to_nat (to_Z (no / 256))))) +
+       Int63.Uint63.of_nat (nat_of_ascii (ascii_of_nat (Z.to_nat (to_Z (no mod 256))))))%sint63  = no.
+Proof.
+  intros.
+  unfold is_two_byte in H.
+  decompose [and] H.
+  assert (to_Z 256 = 256%Z) as to256. { 
+    now compute.
+  }
+  rewrite nat_ascii_embedding.
+  rewrite nat_ascii_embedding.
+  * rewrite add_of_Z.
+    rewrite div_spec;[|right;now compute].
+    rewrite ZifyInst.of_nat_to_nat_eq.
+    rewrite ZifyInst.of_nat_to_nat_eq.
+    rewrite mod_spec.
+    rewrite max_zero_rem;auto.
+    rewrite max_zero_quot;auto.
+    rewrite <- is_int.
+    **  assert (
+            to_Z (256 * of_Z (to_Z no ÷ to_Z 256)) =
+              (to_Z 256) * (to_Z no ÷ to_Z 256))%Z as tvs.
+        {
+          assert (to_Z no ÷ to_Z 256 < 256)%Z.
+          {
+            apply Z.quot_lt_upper_bound; try lia.
+          }
+          assert (256 < Z.pow_pos 2 63 / 2)%Z by now compute.
+          assert (0 <= to_Z no ÷ to_Z 256)%Z. {
+            rewrite to256.
+            apply Z.quot_le_lower_bound; lia.
+          }
+          rewrite to_Z_mul.
+          -  rewrite of_Z_spec.
+             replace (cmod (to_Z no ÷ to_Z 256) wB)%Z with (to_Z no ÷ to_Z 256)%Z.
+             auto.
+             rewrite cmod_small.
+             auto.
+             split.
+             -- simpl.
+                lia.
+             -- unfold wB.
+                unfold size.
+                simpl.
+                lia.
+          - split.
+            -- assert (0 <= to_Z 256 * to_Z (of_Z (to_Z no ÷ to_Z 256)))%Z. {
+                 rewrite to256.
+                 rewrite of_Z_spec.
+                 apply Z.mul_nonneg_nonneg; try lia.
+                 rewrite cmod_small.
+                 + apply Z.quot_pos; try lia.
+                 + split.
+                   ++ rewrite to256 in *.
+                      simpl.
+                      lia.
+                   ++ rewrite to256 in *.
+                      unfold wB.
+                      simpl.
+                      lia.
+               }
+               replace (to_Z min_int) with  (-4611686018427387904)%Z by now compute.
+               lia.
+            -- rewrite to256.
+               assert (to_Z (of_Z (to_Z no ÷ 256)) <= 256)%Z. {
+                 replace   (to_Z (of_Z (to_Z no ÷ 256))) with (cmod (to_Z no ÷ 256) wB)
+                   by now rewrite of_Z_spec.
+                 rewrite cmod_small.
+                 + apply Z.quot_le_upper_bound; try lia.
+                 + split.
+                   ++ unfold wB.
+                      simpl.
+                      rewrite <- to256.
+                      lia.
+                   ++ rewrite <- to256.
+                      unfold wB.
+                      simpl.
+                      lia.
+               }
+               assert ( 256 * to_Z (of_Z (to_Z no ÷ 256)) <= 256*256)%Z. {
+                 apply Z.mul_le_mono_nonneg_l;lia.
+               }
+               assert (256 * 256 <= to_Z max_int)%Z by now compute.
+               lia.
+        }
+        rewrite tvs.
+        rewrite to256.
+        rewrite <- Z.quot_rem'.
+        now rewrite of_to_Z.
+    ** split.
+       *** assert (0 <= Z.rem (to_Z no) (to_Z 256))%Z.
+           {apply  Z.rem_nonneg;auto.
+            rewrite to256.
+            congruence.
+           }
+           generalize abs_int_low;intros.
+           lia.
+       *** generalize Z.rem_bound_pos_pos;intros.
+           assert (2 ^ 16 - 1 <= to_Z max_int)%Z. {
+             unfold max_int.
+             now compute.
+           }
+           assert ((to_Z no) <= to_Z max_int)%Z by lia.
+           assert (0 <=Z.rem (to_Z no) (to_Z 256) <  (to_Z 256))%Z by (apply H2;auto;lia).
+           rewrite to256 in *.
+           assert (256 <= to_Z max_int)%Z by now compute.
+           lia.
+  * assert (to_Z (no mod 256) < 256%Z)%Z. {
+      rewrite mod_spec.
+      apply Z.rem_bound_pos_pos; lia.
+    }
+    replace 256 with (Z.to_nat 256) by now compute.
+    lia.
+  * assert (to_Z (no / 256) < 256%Z)%Z. {
+      rewrite div_spec.
+      apply Z.quot_lt_upper_bound; try lia.
+      right; congruence.
+    } 
+    replace 256 with (Z.to_nat 256) by now compute.
+    lia.
+Qed.
